syntax_processor : initial work

formal_av1.v
@@ -1,18 +1,18 @@
-(* 
+(*
  * Copyright 2018 Dominik Wójt
- * 
+ *
  * This file is part of formal_av1.
- * 
+ *
  * formal_av1 is free software: you can redistribute it and/or modify
  * it under the terms of the GNU General Public License as published by
  * the Free Software Foundation, either version 3 of the License, or
  * (at your option) any later version.
- * 
+ *
  * formal_av1 is distributed in the hope that it will be useful,
  * but WITHOUT ANY WARRANTY; without even the implied warranty of
  * MERCHANTABILITY or FITNESS FOR A PARTICULAR PURPOSE.  See the
  * GNU General Public License for more details.
- * 
+ *
  * You should have received a copy of the GNU General Public License
  * along with formal_av1.  If not, see <http://www.gnu.org/licenses/>.
  *
@@ -24,29 +24,50 @@ Import ListNotations.
 Require Import basic_types.
 Require Import pseudocodes.
 Require Import parser.
-
-Module Syntax_processor.
-
-Definition definitionsE :=
-  (map Parser.parse_pseudocode syntax_pseudocodes).
-
-Theorem all_definitions_parsed :
-  forallb
-    (
-      fun x => match x with
-      | Parser.SomeE (_, []) => true
-      | _ => false
-      end)
-    definitionsE = true.
-Proof. reflexivity. Qed.
-
-Definition state := Parser.token -> Z.
-
-Reserved Notation "e '\\' n" (at level 50, left associativity).
-
-End Syntax_processor.
+Require Import syntax_processor.
 
 Inductive bit := bit_0 | bit_1.
 Inductive byte :=
   byte_intro : forall (_ _ _ _ _ _ _ _ : bit), byte.
-Definition bytestream := list byte.
+Definition open_bitstream_unit := list byte.
+
+Section frame_def.
+Open Scope Z_scope.
+Inductive frame :=
+  | frame_intro :
+    forall (width height planes : Z),
+      (0 < width) -> (0 < height) -> (0 < planes) ->
+      (
+        forall (x y c : Z),
+          (0 <= x < width) -> (0 <= y < height) -> (0 <= c < planes) -> Z) ->
+        frame.
+End frame_def.
+
+Definition tile := frame.
+
+(* Ordering of OBUs *)
+
+(* Inductive temporal_unit :=
+  | temporal_unit_intro :
+    temporal_delimiter ->
+    list sequence_header ->
+    list metadata_obu ->
+    (frame_header * list tile_group_obu * list padding_obu) ->
+    list (frame_header * list tile_group_obu * list padding_obu) ->
+    temporal_unit.
+Inductive coded_video_sequence :=
+  | coded_video_sequence_intro :
+    temporal_unit -> list temporal unit -> coded_video_sequence.
+Inductive bitstream :=
+  | bistream_intro :
+    coded_video_sequece -> list coded_video_sequece -> bitstream. *)
+
+(* The final definitions! *)
+
+Inductive general_decode_relation :
+    list open_bitstream_unit -> list frame -> Prop := (* TODO *).
+
+Inductive large_scale_tile_input := (* TODO *).
+Inductive large_scale_tile_decode_relation :
+    large_scale_tile_input -> list tile -> Prop := (* TODO *).
+
