syntax_processor.v
@@ -1,0 +1,56 @@
+Require Import List ZArith.
+Import ListNotations.
+
+Require Import basic_types.
+Require Import pseudocodes.
+Require Import parser.
+(* Maps are copied from logical foundations.
+   TODO: Might want to replace with FMapAVL. *)
+Require Import Maps.
+
+Module syntax_processor.
+
+Definition definitionsE :=
+  (map Parser.parse_pseudocode all_pseudocodes).
+
+Theorem all_definitions_parsed :
+  forallb
+    (
+      fun x => match x with
+      | Parser.SomeE (_, []) => true
+      | _ => false
+      end)
+    definitionsE = true.
+Proof. reflexivity. Qed.
+
+(* An identifier may refere to either a single variable, array of variables,
+   or declaration (of function, of constant or of array of constants). *)
+Inductive value :=
+  | val_variable : Z -> value
+  | val_array : (list Z -> Z) -> value
+  | val_decl : declaration -> value.
+Definition state := partial_map value.
+
+Example state_update_notation_ex0 :
+  empty & {{ "a"%string --> (val_variable 3) }} "a"%string = Some (val_variable 3).
+Proof. reflexivity. Qed.
+
+Reserved Notation "e '//' st '\\' st' \\ x" (at level 50, left associativity).
+Reserved Notation "s '/' st '\\' st'" (at level 40, st at level 39).
+
+(* TODO: add more rules *)
+Inductive
+  eval_stmt : statement -> state -> state -> Prop :=
+  | eval_stmt_expression :
+    forall st st' e v,
+      e // st \\ st' \\ v ->
+      stmt_expression e / st \\ st'
+with
+  eval_expr : expression -> state -> state -> value -> Prop :=
+  | eval_expr_number :
+    forall st x,
+      expr_number x // st \\ st \\ val_variable x
+where "c '/' st '\\' st'" := (eval_stmt c st st')
+and "e '//' st '\\' st' '\\' v" := (eval_expr e st st' v).
+
+End syntax_processor.
